updates

Veritas.Verifier.fst
@@ -8,49 +8,7 @@ open Veritas.Memory
 open Veritas.BinTree
 open Veritas.BinTreePtr
 open Veritas.MerkleAddr
-
-(* Size of a hash value *)
-let hash_size = 256
-
-(* hash_value - bit vector of a specified size *)
-type hash_value = bv_t hash_size
-
-(* 
- * information stored in a merkle node about a descendant
- * either Empty indicating no descendants or a descendant addr and hash
- * When not empty, there is also a bit storing if the descendant was evicted 
- * into blum scheme
- *)
-type desc_hash = 
-  | Empty: desc_hash
-  | Desc: a:merkle_addr -> h:hash_value -> b:bool -> desc_hash
-
-(* payload of a merkle addr *)
-type merkle_payload = 
-  | SMkLeaf: value:payload -> merkle_payload
-  | SMkInternal: left:desc_hash -> right:desc_hash -> merkle_payload
-
-(* merkle hash function maps a merkle payload to a hash value *)
-val mhashfn (m:merkle_payload): Tot hash_value
-
-let is_payload_of_addr (a:merkle_addr) (p:merkle_payload): Tot bool =
-  if is_merkle_leaf a then SMkLeaf? p 
-  else SMkInternal? p
-
-(* merkle payload type conditioned on the address *)
-type merkle_payload_of_addr (a:merkle_addr) = 
-  p:merkle_payload{is_payload_of_addr a p}
-
-(* An internal node merkle payload *)
-type merkle_payload_internal = p:merkle_payload {SMkInternal? p}
-
-(* get descendant hash of a specified direction (left|right) *)
-let desc_hash_dir (c: bin_tree_dir) (p:merkle_payload_internal): desc_hash = 
-  match c with
-  | Left -> SMkInternal?.left p
-  | Right -> SMkInternal?.right p
-
-
+open Veritas.Verifier.Defs
 
 (*
  * The verifier consumes a log that consists of memory operations and
@@ -62,11 +20,14 @@ let desc_hash_dir (c: bin_tree_dir) (p:merkle_payload_internal): desc_hash =
 (* Each entry of the verifier log *)
 type verifier_log_entry =
   | MemoryOp: o:memory_op -> verifier_log_entry
-  | MAdd: a:merkle_addr -> v:merkle_payload -> a':merkle_addr -> verifier_log_entry
-  | MEvict: a:merkle_addr -> a':merkle_addr -> verifier_log_entry
+  | AddM: a:merkle_addr -> v:merkle_payload -> a':merkle_addr -> verifier_log_entry
+  | EvictM: a:merkle_addr -> a':merkle_addr -> verifier_log_entry
 
-
+(* single verifier log *)
 type verifier_log = seq verifier_log_entry
 
 (* index in the verifier log *)
 type vl_index (l:verifier_log) = seq_index l
+
+(* verifier state is a subset of merkle_addr, merkle_payloads *)
+type verifier_state = (a:merkle_addr) -> option (merkle_payload_of_addr a)
