Veritas.MultiSet.fst
@@ -1,0 +1,10 @@
+module Veritas.MultiSet
+
+let mset (a:eqtype):Type0 = admit()
+
+let equal (#a:eqtype) (s1:mset a) (s2:mset a): Tot bool = admit()
+
+let mem (#a:eqtype) (x:a) (s:mset a): Tot nat = admit()
+
+(* empty set *)
+let empty (#a:eqtype): Tot (mset a) = admit()
