Veritas.MultiSet.fsti
@@ -1,0 +1,13 @@
+module Veritas.MultiSet
+
+val mset (a:eqtype): Type0
+
+val equal (#a:eqtype) (s1:mset a) (s2:mset a): Tot bool
+
+(* membership: how many copies of x are in multiset s *)
+val mem (#a:eqtype) (x:a) (s:mset a): Tot nat
+
+(* empty set *)
+val empty (#a:eqtype): Tot (mset a)
+
+
