Veritas.Verifier.Defs.fst
@@ -1,0 +1,5 @@
+module Veritas.Verifier.Defs
+
+let hashfn (m:merkle_payload): hash_value = admit()
+
+let empty_hash_value = zero_vec 
