Veritas.Verifier.Defs.fsti
@@ -1,0 +1,51 @@
+module Veritas.Verifier.Defs
+
+open FStar.BitVector
+open Veritas.BinTree
+open Veritas.MerkleAddr
+open Veritas.Memory
+
+(* size of a hash value *)
+let hash_size = 256
+
+(* hash value *)
+type hash_value = bv_t hash_size
+
+type desc_hash = 
+  | Empty: desc_hash
+  | Desc: a:merkle_addr -> h:hash_value -> b:bool -> desc_hash
+
+type merkle_payload = 
+  | MkLeaf: value: payload -> merkle_payload
+  | MkInternal: left: desc_hash -> right: desc_hash -> merkle_payload
+
+let is_payload_of_addr (a:merkle_addr) (p:merkle_payload): Tot bool = 
+  if is_merkle_leaf a then MkLeaf? p
+  else MkInternal? p
+
+(* merkle payload type conditioned on address *)
+type merkle_payload_of_addr (a:merkle_addr) = 
+  p:merkle_payload{is_payload_of_addr a p}
+
+(* payload of an internal node *)
+type merkle_payload_internal = p:merkle_payload { MkInternal? p }
+
+(* get the descendant hash of a specified direction *)
+let desc_hash_dir (c: bin_tree_dir) (p:merkle_payload_internal): desc_hash = 
+  match c with
+  | Left -> MkInternal?.left p
+  | Right -> MkInternal?.right p
+
+(* hash function maps a merkle payload to a hash value *)
+val hashfn (m:merkle_payload): Tot hash_value
+
+(* timestamps for blum hashing *)
+type timestamp = 
+  | MkTimestamp: epoch: nat -> counter: nat -> timestamp
+
+(* multi-set hash value *)
+type ms_hash_value = hash_value
+
+(* Hash value of an empty set *)
+val empty_hash_value: ms_hash_value
+
